Swap variable generation order; add inline comments
This swaps the order of variable generation so that the outer most
variable is generated first (as opposed to innermost).
Meta-optimization relies on this implicit property to be effective
when optimizing out shared conditions.

Additionally add inline comments to the Rules data structure
and subsequent generated Java so that the rule source
is clear in the generated Java.

Optimizations/DSL/CodeGenAltAlt.thy
@@ -506,17 +506,18 @@ inductive lower :: "PatternExpr \<Rightarrow> VarName set \<Rightarrow> MATCH \<
   ConstantPattern:
   "v' = fresh_var \<Sigma> \<Longrightarrow> (ConstantExprPattern c, \<Sigma>) \<leadsto> (match v' (ConstantPattern c), v', \<Sigma> \<union> {v'})" |
   UnaryPattern:
-  "\<lbrakk>(x, \<Sigma>) \<leadsto> (m\<^sub>x, v\<^sub>x, \<Sigma>\<^sub>x);
-    v' = fresh_var \<Sigma>\<^sub>x\<rbrakk>
-  \<Longrightarrow> (UnaryExprPattern op x, \<Sigma>) \<leadsto> (match v' (UnaryPattern op v\<^sub>x) && m\<^sub>x, v', \<Sigma>\<^sub>x \<union> {v'})" |
+  "\<lbrakk>v' = fresh_var \<Sigma>;
+    (x, \<Sigma> \<union> {v'}) \<leadsto> (m\<^sub>x, v\<^sub>x, \<Sigma>\<^sub>x)\<rbrakk>
+  \<Longrightarrow> (UnaryExprPattern op x, \<Sigma>) \<leadsto> (match v' (UnaryPattern op v\<^sub>x) && m\<^sub>x, v', \<Sigma>\<^sub>x)" |
   BinaryPattern:
-  "\<lbrakk>(x, \<Sigma>) \<leadsto> (m\<^sub>x, v\<^sub>x, \<Sigma>\<^sub>x); (y, \<Sigma>\<^sub>x) \<leadsto> (m\<^sub>y, v\<^sub>y, \<Sigma>\<^sub>y);
-    v' = fresh_var \<Sigma>\<^sub>y\<rbrakk>
-  \<Longrightarrow> (BinaryExprPattern op x y, \<Sigma>) \<leadsto> (match v' (BinaryPattern op v\<^sub>x v\<^sub>y) && m\<^sub>x && m\<^sub>y, v', \<Sigma>\<^sub>y \<union> {v'})" |
+  "\<lbrakk>v' = fresh_var \<Sigma>;
+    (x, \<Sigma> \<union> {v'}) \<leadsto> (m\<^sub>x, v\<^sub>x, \<Sigma>\<^sub>x); (y, \<Sigma>\<^sub>x) \<leadsto> (m\<^sub>y, v\<^sub>y, \<Sigma>\<^sub>y)\<rbrakk>
+  \<Longrightarrow> (BinaryExprPattern op x y, \<Sigma>) \<leadsto> (match v' (BinaryPattern op v\<^sub>x v\<^sub>y) && m\<^sub>x && m\<^sub>y, v', \<Sigma>\<^sub>y)" |
   ConditionalPattern:
-  "\<lbrakk>(c, \<Sigma>) \<leadsto> (m\<^sub>c, v\<^sub>c, \<Sigma>\<^sub>c); (t, \<Sigma>\<^sub>c) \<leadsto> (m\<^sub>t, v\<^sub>t, \<Sigma>\<^sub>t);
-    (f, \<Sigma>\<^sub>t) \<leadsto> (m\<^sub>f, v\<^sub>f, \<Sigma>\<^sub>f); v' = fresh_var \<Sigma>\<^sub>f\<rbrakk>
-  \<Longrightarrow> (ConditionalExprPattern c t f, \<Sigma>) \<leadsto> (match v' (ConditionalPattern v\<^sub>c v\<^sub>t v\<^sub>f) && m\<^sub>c && m\<^sub>t && m\<^sub>f, v', \<Sigma>\<^sub>f \<union> {v'})" |
+  "\<lbrakk>v' = fresh_var \<Sigma>;
+    (c, \<Sigma> \<union> {v'}) \<leadsto> (m\<^sub>c, v\<^sub>c, \<Sigma>\<^sub>c); (t, \<Sigma>\<^sub>c) \<leadsto> (m\<^sub>t, v\<^sub>t, \<Sigma>\<^sub>t);
+    (f, \<Sigma>\<^sub>t) \<leadsto> (m\<^sub>f, v\<^sub>f, \<Sigma>\<^sub>f)\<rbrakk>
+  \<Longrightarrow> (ConditionalExprPattern c t f, \<Sigma>) \<leadsto> (match v' (ConditionalPattern v\<^sub>c v\<^sub>t v\<^sub>f) && m\<^sub>c && m\<^sub>t && m\<^sub>f, v', \<Sigma>\<^sub>f)" |
 
   ConstantVariableUnseen:
   "\<lbrakk>vn \<notin> \<Sigma>; v' = fresh_var \<Sigma>\<rbrakk> \<Longrightarrow> (ConstantVarPattern vn, \<Sigma>) \<leadsto> (match v' (ConstantVariablePattern vn), v', \<Sigma> \<union> {vn, v'})" | 
@@ -604,39 +605,42 @@ next
   then show ?case
     by (simp add: freshness)
 next
-  case (UnaryPattern x \<Sigma> m\<^sub>x v\<^sub>x \<Sigma>\<^sub>x v' op)
+  case (UnaryPattern v' \<Sigma> x m\<^sub>x v\<^sub>x \<Sigma>\<^sub>x op)
   have ih: "\<Sigma> \<inter> ({v\<^sub>x} \<union> use_vars m\<^sub>x \<union> def_vars m\<^sub>x) = {}"
-    using UnaryPattern by presburger
+    using UnaryPattern by blast
   have seq: "({v'} \<union> use_vars (match v' (UnaryPattern op v\<^sub>x) && m\<^sub>x) \<union> def_vars (match v' (UnaryPattern op v\<^sub>x) && m\<^sub>x)) 
     = {v'} \<union> use_vars m\<^sub>x \<union> {v\<^sub>x} \<union> def_vars m\<^sub>x"
     by simp
   then show ?case
-    by (metis UnaryPattern Int_insert_right UnCI Un_assoc Un_commute freshness insert_is_Un lower_finite lower_sigma_update)
+    using UnaryPattern.hyps(1) UnaryPattern.prems freshness ih by auto
 next
-  case (BinaryPattern x \<Sigma> m\<^sub>x v\<^sub>x \<Sigma>\<^sub>x y m\<^sub>y v\<^sub>y \<Sigma>\<^sub>y v' op)
+  case (BinaryPattern v' \<Sigma> x m\<^sub>x v\<^sub>x \<Sigma>\<^sub>x y m\<^sub>y v\<^sub>y \<Sigma>\<^sub>y op)
   have ihx: "\<Sigma> \<inter> ({v\<^sub>x} \<union> use_vars m\<^sub>x \<union> def_vars m\<^sub>x) = {}"
     using BinaryPattern by blast
   have ihy: "\<Sigma>\<^sub>x \<inter> ({v\<^sub>y} \<union> use_vars m\<^sub>y \<union> def_vars m\<^sub>y) = {}"
-    using BinaryPattern lower_finite by presburger
+    using BinaryPattern lower_finite 
+    by (meson finite.emptyI finite.insertI finite_UnI)
   then have ihy': "(\<Sigma> \<union> {v\<^sub>x} \<union> def_vars m\<^sub>x) \<inter> ({v\<^sub>y} \<union> use_vars m\<^sub>y \<union> def_vars m\<^sub>y) = {}"
-    using BinaryPattern lower_sigma_update by presburger
+    using BinaryPattern lower_sigma_update
+    by (smt (verit) Un_commute Un_empty_right Un_insert_right insert_disjoint(2))
   have seq: "({v'} \<union> use_vars (match v' (BinaryPattern op v\<^sub>x v\<^sub>y) && m\<^sub>x && m\<^sub>y) \<union> def_vars (match v' (BinaryPattern op v\<^sub>x v\<^sub>y) && m\<^sub>x && m\<^sub>y))
     = {v'} \<union> use_vars m\<^sub>x \<union> use_vars m\<^sub>y \<union> {v\<^sub>x, v\<^sub>y} \<union> def_vars m\<^sub>x \<union> def_vars m\<^sub>y"
     by force
   then show ?case using seq ihx ihy' apply simp
-    by (smt (verit) BinaryPattern.hyps(1) BinaryPattern.hyps(2) BinaryPattern.hyps(3) BinaryPattern.prems Un_iff disjoint_iff_not_equal freshness lower_finite lower_sigma_update)
+    by (simp add: BinaryPattern.hyps(1) BinaryPattern.prems Int_Un_distrib Int_Un_distrib2 freshness)
 next
-  case (ConditionalPattern c \<Sigma> m\<^sub>c v\<^sub>c \<Sigma>\<^sub>c t m\<^sub>t v\<^sub>t \<Sigma>\<^sub>t f m\<^sub>f v\<^sub>f \<Sigma>\<^sub>f v')
+  case (ConditionalPattern v' \<Sigma> c m\<^sub>c v\<^sub>c \<Sigma>\<^sub>c t m\<^sub>t v\<^sub>t \<Sigma>\<^sub>t f m\<^sub>f v\<^sub>f \<Sigma>\<^sub>f)
   have ihc: "\<Sigma> \<inter> ({v\<^sub>c} \<union> use_vars m\<^sub>c \<union> def_vars m\<^sub>c) = {}"
     using ConditionalPattern by auto
   have iht: "\<Sigma>\<^sub>c \<inter> ({v\<^sub>t} \<union> use_vars m\<^sub>t \<union> def_vars m\<^sub>t) = {}"
-    using ConditionalPattern lower_finite by blast
+    using ConditionalPattern lower_finite 
+    by (meson finite.emptyI finite.insertI finite_UnI)
   have ihf: "\<Sigma>\<^sub>t \<inter> ({v\<^sub>f} \<union> use_vars m\<^sub>f \<union> def_vars m\<^sub>f) = {}"
-    by (meson ConditionalPattern lower_finite)
+    by (metis ConditionalPattern.IH(3) ConditionalPattern.hyps(2) ConditionalPattern.hyps(3) ConditionalPattern.prems finite.emptyI finite.insertI finite_UnI lower_finite)
   have iht': "(\<Sigma> \<union> {v\<^sub>c} \<union> def_vars m\<^sub>c) \<inter> ({v\<^sub>t} \<union> use_vars m\<^sub>t \<union> def_vars m\<^sub>t) = {}"
-    using ConditionalPattern iht lower_sigma_update by presburger
+    using ConditionalPattern.hyps(2) iht lower_sigma_update by fastforce
   then have ihf': "(\<Sigma> \<union> {v\<^sub>c} \<union> def_vars m\<^sub>c \<union> {v\<^sub>t} \<union> def_vars m\<^sub>t) \<inter> ({v\<^sub>f} \<union> use_vars m\<^sub>f \<union> def_vars m\<^sub>f) = {}"
-    using ConditionalPattern ihf lower_sigma_update by presburger
+    by (smt (verit, del_insts) ConditionalPattern.hyps(2) ConditionalPattern.hyps(3) Un_empty_right Un_insert_left Un_insert_right ihf insert_disjoint(2) lower_sigma_update)
   have seq: "({v'} \<union> use_vars (match v' (ConditionalPattern v\<^sub>c v\<^sub>t v\<^sub>f) && m\<^sub>c && m\<^sub>t && m\<^sub>f) \<union> def_vars (match v' (ConditionalPattern v\<^sub>c v\<^sub>t v\<^sub>f) && m\<^sub>c && m\<^sub>t && m\<^sub>f))
     = {v'} \<union> use_vars m\<^sub>c \<union> use_vars m\<^sub>t \<union> use_vars m\<^sub>f \<union> {v\<^sub>c, v\<^sub>t, v\<^sub>f} \<union> def_vars m\<^sub>c \<union> def_vars m\<^sub>t \<union> def_vars m\<^sub>f"
     by (simp add: Un_assoc)
@@ -662,6 +666,12 @@ next
     by (metis Int_empty_right Int_insert_right_if0 UnCI Un_insert_right def_vars.simps(1) def_vars.simps(2) def_vars.simps(3) finite_insert freshness pattern_variables.simps(6) sup_bot_right use_vars.simps(1) use_vars.simps(2) use_vars.simps(3))
 qed
 
+lemma lower_fresh_variable:
+  assumes "finite \<Sigma>"
+  assumes "(e, \<Sigma>) \<leadsto> (m, v, \<Sigma>')"
+  shows "v \<notin> \<Sigma>"
+  using assms(2,1) apply (induction rule: lower.induct) by (simp add:freshness)+
+
 lemma lower_valid_matches:
   assumes "finite \<Sigma>"
   assumes "\<forall>v \<Sigma>. v = fresh_var \<Sigma> \<longrightarrow> v \<notin> \<L> e"
@@ -677,55 +687,61 @@ next
 next
   case (ConstantPattern v' \<Sigma> c)
   then show ?case by simp
+next       
+  case (UnaryPattern v' \<Sigma> x m\<^sub>x v\<^sub>x \<Sigma>\<^sub>x op)
+  have vm: "valid_match m\<^sub>x"
+    using UnaryPattern.IH UnaryPattern.prems(1) UnaryPattern.prems(2) by force
+  have "v' \<noteq> v\<^sub>x" using lower_fresh_variable
+    by (metis Un_insert_right UnaryPattern.hyps(2) UnaryPattern.prems(2) finite_insert insertI1 sup_bot.right_neutral)
+  then have "v' \<notin> pattern_variables (UnaryPattern op v\<^sub>x) \<and> valid_patternx (UnaryPattern op v\<^sub>x)"
+    by simp
+  then show ?case using vm
+    by (metis Int_empty_left MATCH.simps(3) MATCH.simps(9) UnCI Un_insert_right UnaryPattern.prems(2) finite.emptyI finite.insertI finite_UnI insert_disjoint(2) local.UnaryPattern(2) lower_sigma_update2 use_vars.simps(1) valid_match.elims(3) valid_match.simps(1))
 next
-  case (UnaryPattern x \<Sigma> m\<^sub>x v\<^sub>x \<Sigma>\<^sub>x v' op)
-  have "fresh_var \<Sigma>\<^sub>x \<noteq> v\<^sub>x"
-    using lower_sigma_update UnaryPattern freshness
-    by (metis UnCI insertCI lower_finite)
-  have "fresh_var \<Sigma>\<^sub>x \<noteq> v\<^sub>x \<and> fresh_var \<Sigma>\<^sub>x \<notin> def_vars m\<^sub>x"
-    by (metis "UnaryPattern.hyps"(1) "UnaryPattern.prems"(2) UnCI \<open>fresh_var \<Sigma>\<^sub>x \<noteq> v\<^sub>x\<close> freshness lower_finite lower_sigma_update)
-  then show ?case using UnaryPattern by simp
-next
-  case (BinaryPattern x \<Sigma> m\<^sub>x v\<^sub>x \<Sigma>\<^sub>x y m\<^sub>y v\<^sub>y \<Sigma>\<^sub>y v' op)
+  case (BinaryPattern v' \<Sigma> x m\<^sub>x v\<^sub>x \<Sigma>\<^sub>x y m\<^sub>y v\<^sub>y \<Sigma>\<^sub>y op)
   have vmx: "valid_match m\<^sub>x"
     using BinaryPattern by fastforce
   have vmy: "valid_match m\<^sub>y"
-    using BinaryPattern lower_finite
-    by (metis UnCI \<L>_PatternExpr_def vars.simps(5))
-  have "fresh_var \<Sigma>\<^sub>y \<noteq> v\<^sub>x" using BinaryPattern
-    by (metis UnCI freshness insertCI lower_finite lower_sigma_update)
-  also have "fresh_var \<Sigma>\<^sub>y \<noteq> v\<^sub>y" using BinaryPattern
-    by (metis UnCI freshness insertCI lower_finite lower_sigma_update)
+    using BinaryPattern lower_finite using UnCI \<L>_PatternExpr_def vars.simps(5)
+    by (metis finite.emptyI finite_UnI finite_insert)
+  have "v' \<noteq> v\<^sub>x" using BinaryPattern
+    by (meson UnCI finite.emptyI finite.insertI finite_UnI insertCI lower_fresh_variable)
+  also have "v' \<noteq> v\<^sub>y" using BinaryPattern
+    by (metis UnCI finite.emptyI finite.insertI finite_UnI insertCI lower_finite lower_fresh_variable lower_sigma_update)
   moreover have "use_vars m\<^sub>x \<inter> def_vars m\<^sub>y = {}" using BinaryPattern lower_sigma_update2
-    by (metis UnCI disjoint_iff_not_equal lower_finite lower_sigma_update1)
+    by (smt (verit, del_insts) Int_Un_distrib Int_Un_distrib2 Un_empty finite.emptyI finite.insertI finite_UnI lower_finite lower_sigma_update1)
   moreover have "v\<^sub>x \<noteq> v\<^sub>y" using BinaryPattern
-    by (metis Un_commute Un_insert_right disjoint_insert(2) insertI1 lower_finite lower_sigma_update lower_sigma_update2)
-  ultimately have "fresh_var \<Sigma>\<^sub>y \<noteq> v\<^sub>x \<and> fresh_var \<Sigma>\<^sub>y \<noteq> v\<^sub>y \<and> v\<^sub>x \<noteq> v\<^sub>y \<and> use_vars m\<^sub>x \<inter> def_vars m\<^sub>y = {} \<and> fresh_var \<Sigma>\<^sub>y \<notin> def_vars m\<^sub>x \<and> fresh_var \<Sigma>\<^sub>y \<notin> def_vars m\<^sub>y"
-    by (metis BinaryPattern.hyps(1,2) BinaryPattern.prems(2) UnCI freshness lower_finite lower_sigma_update)
+    by (metis UnCI finite.emptyI finite.insertI finite_UnI insertCI lower_finite lower_fresh_variable lower_sigma_update)
+  ultimately have "v' \<noteq> v\<^sub>x \<and> v' \<noteq> v\<^sub>y \<and> v\<^sub>x \<noteq> v\<^sub>y \<and> use_vars m\<^sub>x \<inter> def_vars m\<^sub>y = {} \<and> v' \<notin> def_vars m\<^sub>x \<and> v' \<notin> def_vars m\<^sub>y"
+    by (smt (verit, del_insts) BinaryPattern.hyps(2) BinaryPattern.hyps(3) BinaryPattern.prems(2) Set.set_insert UnCI Un_insert_right disjoint_insert(2) finite.emptyI finite.insertI finite_UnI insert_iff lower_finite lower_sigma_update lower_sigma_update2)
   then show ?case
     by (simp add: BinaryPattern.hyps(3) vmx vmy)
 next
-  case (ConditionalPattern c \<Sigma> m\<^sub>c v\<^sub>c \<Sigma>\<^sub>c t m\<^sub>t v\<^sub>t \<Sigma>\<^sub>t f m\<^sub>f v\<^sub>f \<Sigma>\<^sub>f v')
+  case (ConditionalPattern v' \<Sigma> c m\<^sub>c v\<^sub>c \<Sigma>\<^sub>c t m\<^sub>t v\<^sub>t \<Sigma>\<^sub>t f m\<^sub>f v\<^sub>f \<Sigma>\<^sub>f)
   have vmc: "valid_match m\<^sub>c"
     using ConditionalPattern by force
-  have vmt: "valid_match m\<^sub>t"
-    using ConditionalPattern lower_finite by auto
+  have f: "finite (\<Sigma> \<union> {v'})"
+    using ConditionalPattern.prems(2) by blast
+  then have vmt: "valid_match m\<^sub>t"
+    using ConditionalPattern lower_finite \<L>_PatternExpr_def vars.simps(6)
+    by (metis UnCI)
   have vmf: "valid_match m\<^sub>f"
-    by (metis \<L>_PatternExpr_def ConditionalPattern.IH(3) ConditionalPattern.hyps(1,2) ConditionalPattern.prems(1,2) UnI2 vars.simps(6) lower_finite)
+    using ConditionalPattern lower_finite \<L>_PatternExpr_def vars.simps(6)
+    by (metis UnCI f)
   have v'ne: "v' \<noteq> v\<^sub>c \<and> v' \<noteq> v\<^sub>t \<and> v' \<noteq> v\<^sub>f"
-    by (smt (verit) ConditionalPattern Un_insert_left Un_insert_right freshness insert_iff lower_finite lower_sigma_update)
+    by (metis ConditionalPattern.hyps(2) ConditionalPattern.hyps(3) ConditionalPattern.hyps(4) Un_iff f insert_iff lower_finite lower_fresh_variable lower_sigma_update)
   have dij: "v\<^sub>c \<noteq> v\<^sub>t \<and> v\<^sub>c \<noteq> v\<^sub>f \<and> v\<^sub>t \<noteq> v\<^sub>f"
     using UnCI Un_insert_left disjoint_insert(2) insertCI lower_finite lower_sigma_update1 lower_sigma_update2
-    by (metis ConditionalPattern.hyps(1,2,3) ConditionalPattern.prems(2))
+    by (metis ConditionalPattern.hyps(2) ConditionalPattern.hyps(3) ConditionalPattern.hyps(4) f)
   have cd: "use_vars m\<^sub>c \<inter> (def_vars m\<^sub>t \<union> def_vars m\<^sub>f) = {}"
-    using ConditionalPattern lower_sigma_update2
+    using ConditionalPattern lower_sigma_update2 f
     by (smt (verit, ccfv_threshold) Un_iff disjoint_iff lower_finite lower_sigma_update1)
   have td: "use_vars m\<^sub>t \<inter> def_vars m\<^sub>f = {}"
-    using ConditionalPattern lower_sigma_update2
+    using ConditionalPattern lower_sigma_update2 f
     by (smt (verit, ccfv_SIG) UnCI disjoint_iff lower_finite lower_sigma_update1)
   have "v' \<notin> def_vars m\<^sub>c \<and> v' \<notin> def_vars m\<^sub>t \<and> v' \<notin> def_vars m\<^sub>f"
-    using ConditionalPattern
-    by (metis UnI1 Un_insert_right freshness insertCI lower_finite lower_sigma_update mk_disjoint_insert)
+    using ConditionalPattern f
+    by (smt (verit, del_insts) Int_iff Un_iff insert_absorb insert_iff insert_not_empty lower_finite lower_sigma_update lower_sigma_update2)
   then show ?case using vmc vmt vmf v'ne dij cd td
     by simp
 next
@@ -1134,7 +1150,7 @@ next
   then show ?case using \<L>_PatternExpr_def
     by (metis vars.simps(4) eval_match_andthen valid_match.simps(2))
 next
-  case (BinaryPattern x \<Sigma> m\<^sub>x v\<^sub>x \<Sigma>\<^sub>x y m\<^sub>y v\<^sub>y \<Sigma>\<^sub>y v' op)
+  case (BinaryPattern v' \<Sigma> x m\<^sub>x v\<^sub>x \<Sigma>\<^sub>x y m\<^sub>y v\<^sub>y \<Sigma>\<^sub>y op)
   obtain \<sigma>\<^sub>m where \<sigma>\<^sub>m: "match v' (BinaryPattern op v\<^sub>x v\<^sub>y) \<U> \<sigma> = \<sigma>\<^sub>m"
     by (meson BinaryPattern.prems eval_match_andthen)
   then obtain \<sigma>\<^sub>x where \<sigma>\<^sub>x: "m\<^sub>x \<U> \<sigma>\<^sub>m = \<sigma>\<^sub>x"
@@ -1142,9 +1158,9 @@ next
   then obtain \<sigma>\<^sub>y where \<sigma>\<^sub>y: "m\<^sub>y \<U> \<sigma>\<^sub>x = \<sigma>\<^sub>y"
     by (metis BinaryPattern.prems(2) \<open>match v' (BinaryPattern op v\<^sub>x v\<^sub>y) \<U> \<sigma> = \<sigma>\<^sub>m\<close> eval_match_andthen eval_match_deterministic)
   have xs: "vars x \<subseteq> dom \<sigma>\<^sub>x"
-    using BinaryPattern.hyps(2) \<sigma>\<^sub>x BinaryPattern.prems(1) by auto
+    using BinaryPattern.hyps(3) BinaryPattern.prems(1) \<sigma>\<^sub>x by auto
   have ys: "vars y \<subseteq> dom \<sigma>\<^sub>y"
-    using BinaryPattern.hyps(4) \<sigma>\<^sub>y BinaryPattern.prems(1) by auto
+    using BinaryPattern.hyps(5) \<sigma>\<^sub>y BinaryPattern.prems(1) by auto
   have "vars (BinaryExprPattern op x y) = \<L> x \<union> \<L> y"
     by simp
   have "dom \<sigma>\<^sub>x \<union> dom \<sigma>\<^sub>y \<subseteq> dom \<sigma>'"
@@ -1152,7 +1168,7 @@ next
   then show ?case
     by (metis Un_subset_iff \<L>_PatternExpr_def \<open>vars (BinaryExprPattern op x y) = \<L> x \<union> \<L> y\<close> sup.absorb_iff1 xs ys)
 next
-  case (ConditionalPattern c \<Sigma> m\<^sub>c v\<^sub>c \<Sigma>\<^sub>c t m\<^sub>t v\<^sub>t \<Sigma>\<^sub>t f m\<^sub>f v\<^sub>f \<Sigma>\<^sub>f v')
+  case (ConditionalPattern v' \<Sigma> c m\<^sub>c v\<^sub>c \<Sigma>\<^sub>c t m\<^sub>t v\<^sub>t \<Sigma>\<^sub>t f m\<^sub>f v\<^sub>f \<Sigma>\<^sub>f)
   obtain \<sigma>\<^sub>m where \<sigma>\<^sub>m: "match v' (ConditionalPattern v\<^sub>c v\<^sub>t v\<^sub>f) \<U> \<sigma> = \<sigma>\<^sub>m"
     by (meson ConditionalPattern.prems eval_match_andthen)
   then obtain \<sigma>\<^sub>c where \<sigma>\<^sub>c: "m\<^sub>c \<U> \<sigma>\<^sub>m = \<sigma>\<^sub>c"
@@ -1162,12 +1178,12 @@ next
   then obtain \<sigma>\<^sub>f where \<sigma>\<^sub>f: "m\<^sub>f \<U> \<sigma>\<^sub>t = \<sigma>\<^sub>f"
     by (metis ConditionalPattern.prems(2) \<sigma>\<^sub>c \<sigma>\<^sub>m eval_match_andthen eval_match_deterministic)
   have cs: "vars c \<subseteq> dom \<sigma>\<^sub>c"
-    using ConditionalPattern.hyps(2) \<sigma>\<^sub>c ConditionalPattern.prems(1) by auto
+    using ConditionalPattern.hyps(3) \<sigma>\<^sub>c ConditionalPattern.prems(1) by auto
   have ts: "vars t \<subseteq> dom \<sigma>\<^sub>t"
-    using ConditionalPattern.hyps(4) \<sigma>\<^sub>t ConditionalPattern.prems(1) by auto
+    using ConditionalPattern.hyps(5) \<sigma>\<^sub>t ConditionalPattern.prems(1) by auto
   have fs: "vars f \<subseteq> dom \<sigma>\<^sub>f"
-    using ConditionalPattern.hyps(4) \<sigma>\<^sub>f ConditionalPattern.prems(1)
-    using ConditionalPattern.hyps(6) by auto
+    using ConditionalPattern.hyps(5) \<sigma>\<^sub>f ConditionalPattern.prems(1)
+    using ConditionalPattern.hyps(7) by auto
   have vu: "vars (ConditionalExprPattern c t f) = \<L> c \<union> \<L> t \<union> \<L> f"
     by simp
   have "dom \<sigma>\<^sub>c \<union> dom \<sigma>\<^sub>t \<union> dom \<sigma>\<^sub>f \<subseteq> dom \<sigma>'"
@@ -1235,7 +1251,7 @@ next
   then show ?case
     by simp
 next
-  case (UnaryPattern x \<Sigma> m\<^sub>x v\<^sub>x \<Sigma>\<^sub>x v' op)
+  case (UnaryPattern v' \<Sigma> x m\<^sub>x v\<^sub>x \<Sigma>\<^sub>x op)
   obtain \<sigma>\<^sub>m where m1: "match v' (UnaryPattern op v\<^sub>x) \<U> \<sigma>(v' \<mapsto> e\<^sub>g) = \<sigma>\<^sub>m"
     by (meson UnaryPattern.prems(3) eval_match_andthen)
   then obtain e\<^sub>x where  e\<^sub>g: "e\<^sub>g = UnaryExpr op e\<^sub>x" using UnaryPattern
@@ -1256,18 +1272,20 @@ next
   then show ?case
     using e\<^sub>g by auto
 next
-  case (BinaryPattern x \<Sigma> m\<^sub>x v\<^sub>x \<Sigma>\<^sub>x y m\<^sub>y v\<^sub>y \<Sigma>\<^sub>y v' op)
+  case (BinaryPattern v' \<Sigma> x m\<^sub>x v\<^sub>x \<Sigma>\<^sub>x y m\<^sub>y v\<^sub>y \<Sigma>\<^sub>y op)
   obtain \<sigma>\<^sub>m where s1: "match v' (BinaryPattern op v\<^sub>x v\<^sub>y) \<U> \<sigma>(v' \<mapsto> e\<^sub>g) = \<sigma>\<^sub>m"
     by (meson BinaryPattern.prems(3) eval_match_andthen)
   then obtain e\<^sub>x e\<^sub>y where e\<^sub>g: "e\<^sub>g = BinaryExpr op e\<^sub>x e\<^sub>y"
     by (meson eval_match_BinaryPattern map_upd_Some_unfold)
+  have f: "finite (\<Sigma> \<union> {v'})"
+    using BinaryPattern.prems(1) by blast
   have u1: "unify (\<sigma>(v' \<mapsto> e\<^sub>g)) [(v\<^sub>x, e\<^sub>x), (v\<^sub>y, e\<^sub>y)] \<sigma>\<^sub>m"
       using e\<^sub>g IRExpr.inject(2) s1 eval_match_BinaryPattern by fastforce
   then obtain \<sigma>\<^sub>x where m1: "m\<^sub>x \<U> \<sigma>\<^sub>m = \<sigma>\<^sub>x"
     by (metis BinaryPattern.prems(3) eval_match_andthen eval_match_deterministic s1)
   then have mx: "\<sigma>\<^sub>m \<subseteq>\<^sub>m \<sigma>\<^sub>x"
-    using BinaryPattern.prems(2) eval_match_subset m1 
-    by (metis BinaryPattern.hyps(1) BinaryPattern.prems(1) lower_valid_matches valid_pattern.simps(5) valid_pattern_preserves_freshness)
+    using BinaryPattern.prems(3) eval_match_subset m1 f
+    by (metis BinaryPattern.hyps(2) BinaryPattern.prems(2) lower_valid_matches valid_pattern.simps(5) valid_pattern_preserves_freshness)
   then have mt1: "match_tree x e\<^sub>x = Some (\<sigma>\<^sub>x |` \<L> x)"
   proof -
     obtain \<sigma>\<^sub>x' where xm: "m\<^sub>x \<U> \<sigma>\<^sub>x'(v\<^sub>x \<mapsto> e\<^sub>x) = \<sigma>\<^sub>x"
@@ -1287,20 +1305,21 @@ next
       using m1 u1 unify_partition
       by (metis list.set_intros(1) m2 unify_unempty)
     then show ?thesis
-      using BinaryPattern
-      using lower_finite by fastforce
+      using BinaryPattern f
+      by (meson lower_finite valid_pattern.simps(5))
   qed
   have comp: "compatible \<sigma>\<^sub>x \<sigma>'" using mx
-    using compatible.elims(3) eval_match_andthen eval_match_deterministic eval_match_subset m1 map_le_def s1 valid_match.simps(4)
-    compatible_alt by (metis BinaryPattern.hyps(1,3) BinaryPattern.prems(1,2,3) lower_finite lower_valid_matches valid_pattern.simps(5) valid_pattern_preserves_freshness)
+    using compatible.elims(3) eval_match_andthen eval_match_deterministic eval_match_subset m1 map_le_def s1 valid_match.simps(4) f
+    compatible_alt 
+    by (metis BinaryPattern lower_finite lower_valid_matches valid_pattern.simps(5) valid_pattern_preserves_freshness)
   then have comp': "compatible (\<sigma>\<^sub>x |` \<L> x) (\<sigma>' |` \<L> y)"
     using compatible_alt by (metis (full_types) domIff restrict_in restrict_out)
   have "\<sigma>\<^sub>x ++ \<sigma>' = \<sigma>'"
-    using mx
-    by (metis BinaryPattern.hyps(1,3) BinaryPattern.prems(1,2,3) eval_match_andthen eval_match_deterministic eval_match_subset lower_finite lower_valid_matches m1 map_add_subsumed1 s1 valid_pattern.simps(5) valid_pattern_preserves_freshness)
+    using mx f
+    by (metis BinaryPattern eval_match_andthen eval_match_deterministic eval_match_subset lower_finite lower_valid_matches m1 map_add_subsumed1 s1 valid_pattern.simps(5) valid_pattern_preserves_freshness)
   have "(dom \<sigma>' - dom \<sigma>\<^sub>x) \<inter> \<L> x = {}" \<comment> \<open>Ian: This is the troublesome case\<close>
-    using eval_match_adds_patterns \<L>_PatternExpr_def
-    by (metis BinaryPattern.hyps(1) BinaryPattern.prems(1,2) DiffD2 disjoint_iff lower_valid_matches m1 subset_eq valid_pattern.simps(5) valid_pattern_preserves_freshness)
+    using eval_match_adds_patterns \<L>_PatternExpr_def f
+    by (metis BinaryPattern DiffD2 disjoint_iff lower_valid_matches m1 subset_eq valid_pattern.simps(5) valid_pattern_preserves_freshness)
   then have "(\<sigma>\<^sub>x |` \<L> x) ++ (\<sigma>' |` \<L> y) = (\<sigma>' |` \<L> x) ++ (\<sigma>' |` \<L> y)"
     using compatible_alt by (metis (no_types, lifting) \<open>\<sigma>\<^sub>x ++ \<sigma>' = \<sigma>'\<close> comp map_add_None map_le_def restricted_unchanged)
   then have "(\<sigma>\<^sub>x |` \<L> x) ++ (\<sigma>' |` \<L> y) = (\<sigma>' |` (vars x \<union> \<L> y))"
@@ -1313,18 +1332,20 @@ next
   then show ?case using mt1 mt2 e\<^sub>g
     by simp
 next
-  case (ConditionalPattern c \<Sigma> m\<^sub>c v\<^sub>c \<Sigma>\<^sub>c t m\<^sub>t v\<^sub>t \<Sigma>\<^sub>t f m\<^sub>f v\<^sub>f \<Sigma>\<^sub>f v')
+  case (ConditionalPattern v' \<Sigma> c m\<^sub>c v\<^sub>c \<Sigma>\<^sub>c t m\<^sub>t v\<^sub>t \<Sigma>\<^sub>t f m\<^sub>f v\<^sub>f \<Sigma>\<^sub>f)
   obtain \<sigma>\<^sub>m where s1: "match v' (ConditionalPattern v\<^sub>c v\<^sub>t v\<^sub>f) \<U> \<sigma>(v' \<mapsto> e\<^sub>g) = \<sigma>\<^sub>m"
     by (meson ConditionalPattern.prems(3) eval_match_andthen)
   then obtain e\<^sub>c e\<^sub>t e\<^sub>f where e\<^sub>g: "e\<^sub>g = ConditionalExpr e\<^sub>c e\<^sub>t e\<^sub>f"
     by (meson eval_match_ConditionalPattern map_upd_Some_unfold)
+  have f: "finite (\<Sigma> \<union> {v'})"
+    using ConditionalPattern.prems(1) by blast
   have u1: "unify (\<sigma>(v' \<mapsto> e\<^sub>g)) [(v\<^sub>c, e\<^sub>c), (v\<^sub>t, e\<^sub>t), (v\<^sub>f, e\<^sub>f)] \<sigma>\<^sub>m"
       using e\<^sub>g IRExpr.inject(2) s1 eval_match_ConditionalPattern by fastforce
   then obtain \<sigma>\<^sub>c where m1: "m\<^sub>c \<U> \<sigma>\<^sub>m = \<sigma>\<^sub>c"
     by (metis ConditionalPattern.prems(3) eval_match_andthen eval_match_deterministic s1)
   then have mx: "\<sigma>\<^sub>m \<subseteq>\<^sub>m \<sigma>\<^sub>c"
-    using ConditionalPattern.prems(2) eval_match_subset m1
-    by (metis ConditionalPattern.hyps(1) ConditionalPattern.prems(1) lower_valid_matches valid_pattern.simps(6) valid_pattern_preserves_freshness)
+    using ConditionalPattern.prems(3) eval_match_subset m1 f
+    by (metis ConditionalPattern lower_valid_matches valid_pattern.simps(6) valid_pattern_preserves_freshness)
   then have mt1: "match_tree c e\<^sub>c = Some (\<sigma>\<^sub>c |` \<L> c)"
   proof -
     obtain \<sigma>\<^sub>c' where xm: "m\<^sub>c \<U> \<sigma>\<^sub>c'(v\<^sub>c \<mapsto> e\<^sub>c) = \<sigma>\<^sub>c"
@@ -1335,15 +1356,16 @@ next
   qed
   obtain \<sigma>\<^sub>t where m2: "m\<^sub>t \<U> \<sigma>\<^sub>c = \<sigma>\<^sub>t"
     by (metis ConditionalPattern.prems(3) eval_match_andthen eval_match_deterministic m1 s1)
-  then have mxt: "\<sigma>\<^sub>c \<subseteq>\<^sub>m \<sigma>\<^sub>t"
-    by (metis ConditionalPattern.hyps(1) ConditionalPattern.hyps(3) ConditionalPattern.prems(1) ConditionalPattern.prems(2) eval_match_subset lower_finite lower_valid_matches valid_pattern.simps(6) valid_pattern_preserves_freshness)
+  then have mxt: "\<sigma>\<^sub>c \<subseteq>\<^sub>m \<sigma>\<^sub>t" using f
+    by (metis ConditionalPattern eval_match_subset lower_finite lower_valid_matches valid_pattern.simps(6) valid_pattern_preserves_freshness)
   then have mt2: "match_tree t e\<^sub>t = Some (\<sigma>\<^sub>t |` \<L> t)"
   proof -
     obtain \<sigma>\<^sub>t' where tm: "m\<^sub>t \<U> \<sigma>\<^sub>t'(v\<^sub>t \<mapsto> e\<^sub>t) = \<sigma>\<^sub>t"
       using m1 m2 u1 unify_partition
       by (metis list.set_intros(1) mx unify_unempty)
     then show ?thesis
-      using ConditionalPattern lower_finite by fastforce
+      using ConditionalPattern lower_finite f
+      by (meson valid_pattern.simps(6))
   qed
   then have mt3: "match_tree f e\<^sub>f = Some (\<sigma>' |` \<L> f)"
   proof -
@@ -1354,13 +1376,13 @@ next
       using m1 m2 u1 unify_partition
       by (meson list.set_intros(1) list.set_intros(2) map_le_trans mx mxt)
     then show ?thesis
-      using ConditionalPattern
+      using ConditionalPattern f
       by (metis \<L>_PatternExpr_def lower_finite valid_pattern.simps(6))
   qed
-  then have mxs: "\<sigma>\<^sub>t \<subseteq>\<^sub>m \<sigma>'"
-    by (metis ConditionalPattern.hyps(1) ConditionalPattern.hyps(3) ConditionalPattern.hyps(5) ConditionalPattern.prems(1) ConditionalPattern.prems(2) ConditionalPattern.prems(3) eval_match_andthen eval_match_deterministic eval_match_subset lower_finite lower_valid_matches m1 m2 s1 valid_pattern.simps(6) valid_pattern_preserves_freshness)
-  have comp: "compatible \<sigma>\<^sub>c \<sigma>'" using mx
-    by (metis ConditionalPattern.hyps(1) ConditionalPattern.hyps(3) ConditionalPattern.hyps(5) ConditionalPattern.prems(1) ConditionalPattern.prems(2) ConditionalPattern.prems(3) compatible_alt eval_match_andthen eval_match_deterministic eval_match_subset lower_finite lower_valid_matches m1 map_le_def map_le_trans s1 valid_pattern.simps(6) valid_pattern_preserves_freshness)
+  then have mxs: "\<sigma>\<^sub>t \<subseteq>\<^sub>m \<sigma>'" using f
+    by (metis ConditionalPattern eval_match_andthen eval_match_deterministic eval_match_subset lower_finite lower_valid_matches m1 m2 s1 valid_pattern.simps(6) valid_pattern_preserves_freshness)
+  have comp: "compatible \<sigma>\<^sub>c \<sigma>'" using mx f
+    by (metis ConditionalPattern compatible_alt eval_match_andthen eval_match_deterministic eval_match_subset lower_finite lower_valid_matches m1 map_le_def map_le_trans s1 valid_pattern.simps(6) valid_pattern_preserves_freshness)
   then have compc: "compatible (\<sigma>\<^sub>c |` \<L> c) (\<sigma>\<^sub>t |` \<L> t)"
     by (smt (verit, best) compatible_alt domIff map_le_def mxt restrict_in restrict_out)
   have compt: "compatible (\<sigma>\<^sub>t |` \<L> t) (\<sigma>' |` \<L> f)"
@@ -1369,19 +1391,20 @@ next
   from comp have comp': "compatible (\<sigma>\<^sub>c |` \<L> c) (\<sigma>' |` \<L> f)"
     using compatible_alt by (metis (full_types) domIff restrict_in restrict_out)
   have "(\<sigma>\<^sub>c ++ \<sigma>\<^sub>t) ++ \<sigma>' = \<sigma>'"
-    using mx
-    by (metis ConditionalPattern.hyps(1) ConditionalPattern.hyps(3) ConditionalPattern.hyps(5) ConditionalPattern.prems(1) ConditionalPattern.prems(2) ConditionalPattern.prems(3) eval_match_andthen eval_match_deterministic eval_match_subset lower_finite lower_valid_matches m1 m2 map_add_subsumed1 s1 valid_pattern.simps(6) valid_pattern_preserves_freshness)
+    using mx f
+    by (metis ConditionalPattern eval_match_andthen eval_match_deterministic eval_match_subset lower_finite lower_valid_matches m1 m2 map_add_subsumed1 s1 valid_pattern.simps(6) valid_pattern_preserves_freshness)
   have "(dom \<sigma>\<^sub>t - dom \<sigma>\<^sub>c) \<inter> \<L> c= {}" \<comment> \<open>Ian: This is the troublesome case\<close>
-    using eval_match_adds_patterns \<L>_PatternExpr_def
-    by (metis ConditionalPattern.hyps(1) ConditionalPattern.prems(1) ConditionalPattern.prems(2) DiffD2 disjoint_iff in_mono lower_valid_matches m1 valid_pattern.simps(6) valid_pattern_preserves_freshness)
+    using eval_match_adds_patterns \<L>_PatternExpr_def f
+    by (metis ConditionalPattern DiffD2 disjoint_iff in_mono lower_valid_matches m1 valid_pattern.simps(6) valid_pattern_preserves_freshness)
   then have tplus: "(\<sigma>\<^sub>c |` \<L> c) ++ (\<sigma>\<^sub>t |` \<L> t) = (\<sigma>\<^sub>t |` \<L> c) ++ (\<sigma>\<^sub>t |` \<L> t)"
     by (simp add: mxt restricted_unchanged)
   have "(dom \<sigma>' - dom \<sigma>\<^sub>t - dom \<sigma>\<^sub>c) \<inter> \<L> t \<inter> \<L> c= {}" \<comment> \<open>Ian: This is the troublesome case\<close>
     using eval_match_adds_patterns
-    using ConditionalPattern.hyps(1) ConditionalPattern.prems(1) ConditionalPattern.prems(2) lower_valid_matches m1 valid_pattern_preserves_freshness by fastforce
+    using ConditionalPattern.hyps(1) ConditionalPattern.prems(1) ConditionalPattern.prems(2) lower_valid_matches m1 valid_pattern_preserves_freshness
+    by (metis ConditionalPattern.hyps(2) Diff_Int_distrib2 Diff_disjoint Int_absorb Int_absorb1 Int_assoc Int_left_commute f valid_pattern.simps(6))
   then have tplus: "(\<sigma>\<^sub>c |` \<L> c) ++ (\<sigma>\<^sub>t |` \<L> t) = (\<sigma>' |` \<L> c) ++ (\<sigma>' |` \<L> t)"
-    using tplus mxs \<L>_PatternExpr_def
-    by (smt (verit, ccfv_threshold) ConditionalPattern.hyps(1) ConditionalPattern.hyps(3) ConditionalPattern.prems(1) ConditionalPattern.prems(2) Diff_disjoint disjoint_iff eval_match_adds_patterns in_mono lower_finite lower_valid_matches m1 m2 map_le_trans mxt restricted_unchanged valid_pattern.simps(6) valid_pattern_preserves_freshness)
+    using tplus mxs \<L>_PatternExpr_def f
+    by (smt (verit, ccfv_threshold) ConditionalPattern Diff_disjoint disjoint_iff eval_match_adds_patterns in_mono lower_finite lower_valid_matches m1 m2 map_le_trans mxt restricted_unchanged valid_pattern.simps(6) valid_pattern_preserves_freshness)
   then have "(\<sigma>\<^sub>c |` \<L> c) ++ ((\<sigma>\<^sub>t |` \<L> t) ++ (\<sigma>' |` \<L> f)) = ((\<sigma>' |` \<L> c) ++ (\<sigma>' |` \<L> t)) ++ (\<sigma>' |` \<L> f)"
     by simp
   then have uadd: "(\<sigma>\<^sub>c |` \<L> c) ++ ((\<sigma>\<^sub>t |` \<L> t) ++ (\<sigma>' |` \<L> f)) = (\<sigma>' |` (\<L> c \<union> \<L> t \<union> \<L> f))"
@@ -1439,12 +1462,69 @@ instance apply standard
   done
 end
 
+definition subif :: "(VarName \<Rightarrow> VarName option) \<Rightarrow> VarName \<Rightarrow> VarName" where
+  "subif \<sigma> v = (case \<sigma> v of Some v' \<Rightarrow> v' | None \<Rightarrow> v)"
+
+instantiation CodePattern :: substitutable begin
+fun substitute_CodePattern :: "CodePattern \<Rightarrow> (VarName \<Rightarrow> VarName option) \<Rightarrow> CodePattern" where
+  "UnaryPattern op v \<Zhide> \<sigma> = 
+    (UnaryPattern op (subif \<sigma> v))" |
+  "BinaryPattern op v1 v2 \<Zhide> \<sigma> = 
+    (BinaryPattern op (subif \<sigma> v1) (subif \<sigma> v2))" |
+  "ConditionalPattern v1 v2 v3 \<Zhide> \<sigma> = 
+    (ConditionalPattern (subif \<sigma> v1) (subif \<sigma> v2) (subif \<sigma> v3))" |
+  "VariablePattern v \<Zhide> \<sigma> = 
+    (VariablePattern (subif \<sigma> v))" |
+  "ConstantPattern val \<Zhide> \<sigma> = 
+    (ConstantPattern val)" |
+  "ConstantVariablePattern v \<Zhide> \<sigma> = 
+    (ConstantVariablePattern (subif \<sigma> v))" |
+  "ParameterPattern val \<Zhide> \<sigma> = 
+    (ParameterPattern val)" |
+  "LeafPattern val \<Zhide> \<sigma> = 
+    (LeafPattern val)"
+instance apply standard
+  subgoal for r apply (induction r)
+    by (simp add: subif_def)+
+  done
+end
+
+instantiation MATCH :: substitutable begin
+fun substitute_MATCH :: "MATCH \<Rightarrow> (VarName \<Rightarrow> VarName option) \<Rightarrow> MATCH" where
+  "match v p \<Zhide> \<sigma> = (match (subif \<sigma> v) (p \<Zhide> \<sigma>))" |
+  "equality v1 v2 \<Zhide> \<sigma> = equality (subif \<sigma> v1) (subif \<sigma> v2)" |
+  "andthen m1 m2 \<Zhide> \<sigma> = andthen (m1 \<Zhide> \<sigma>) (m2 \<Zhide> \<sigma>)" |
+  "condition c \<Zhide> \<sigma> = condition c" | (* TODO: Do we need to substitute in condition? *)
+  "noop v \<Zhide> \<sigma> = noop (subif \<sigma> v)"
+instance apply standard
+  subgoal for r apply (induction r)
+    by (simp add: subif_def identity)+
+  done
+end
+
+type_synonym RuleLabel = "String.literal"
+
+
 datatype Rules =
-  base PatternExpr |
+  base RuleLabel PatternExpr |
   cond MATCH Rules |
   either Rules Rules |
   seq Rules Rules |
   choice "Rules list"
+
+instantiation Rules :: substitutable begin
+fun substitute_Rules :: "Rules \<Rightarrow> (VarName \<Rightarrow> VarName option) \<Rightarrow> Rules" where
+  "base s p \<Zhide> \<sigma> = (base s p)" | (* TODO: Do we need to substitute in pattern expr? *)
+  "cond m r \<Zhide> \<sigma> = (cond (m \<Zhide> \<sigma>) (r \<Zhide> \<sigma>))" |
+  "either r1 r2 \<Zhide> \<sigma> = (either (r1 \<Zhide> \<sigma>) (r2 \<Zhide> \<sigma>))" |
+  "seq r1 r2 \<Zhide> \<sigma> = (seq (r1 \<Zhide> \<sigma>) (r2 \<Zhide> \<sigma>))" |
+  "choice r \<Zhide> \<sigma> = (choice (map (\<lambda>r. r \<Zhide> \<sigma>) r))"
+instance apply standard
+  subgoal for r apply (induction r)
+        apply (simp add: subif_def identity)+
+    by (simp add: list.map_ident_strong)
+  done
+end
 
 bundle match_pattern_syntax begin
 
@@ -1477,14 +1557,14 @@ abbreviation map_filter :: "('a \<Rightarrow> 'b option) \<Rightarrow> 'a list \
 
 fun entry_var :: "Rules \<Rightarrow> VarName option" where
   "entry_var (m ? r) = (case match_entry_var m of Some v \<Rightarrow> Some v | None \<Rightarrow> entry_var r)" |
-  "entry_var (base e) = None" |
+  "entry_var (base s e) = None" |
   "entry_var (r1 else r2) = (case entry_var r1 of Some v \<Rightarrow> Some v | None \<Rightarrow> entry_var r2)" |
   "entry_var (choice xs) = find (\<lambda>_.True) (map_filter entry_var xs)" |
   "entry_var (r1 \<Zsemi> r2) = (case entry_var r1 of Some v \<Rightarrow> Some v | None \<Rightarrow> entry_var r2)"
 
 inductive eval_rules :: "Rules \<Rightarrow> Subst \<Rightarrow> IRExpr option \<Rightarrow> bool" where
   \<comment> \<open>Evaluate the result\<close>
-  "eval_rules (base e) \<sigma> (e $$ \<sigma>)" |
+  "eval_rules (base s e) \<sigma> (e $$ \<sigma>)" |
 
   \<comment> \<open>Evaluate a condition\<close>
   "\<lbrakk>m \<U> \<sigma> = \<sigma>';
@@ -1518,24 +1598,23 @@ inductive eval_rules :: "Rules \<Rightarrow> Subst \<Rightarrow> IRExpr option \
     eval_rules r2 \<sigma> r\<rbrakk>
    \<Longrightarrow> eval_rules (r1 \<Zsemi> r2) \<sigma> r"
 
-inductive_cases baseE: "eval_rules (base e') u e"
+inductive_cases baseE: "eval_rules (base s e') u e"
 inductive_cases condE: "eval_rules (cond m r) u e"
 inductive_cases elseE: "eval_rules (r1 else r2) u e"
 inductive_cases choiceE: "eval_rules (choice r) u e"
 inductive_cases seqE: "eval_rules (r1 \<Zsemi> r2) u e"
 
+inductive generate :: "RuleLabel \<Rightarrow> PatternExpr \<Rightarrow> Condition option \<Rightarrow> PatternExpr \<Rightarrow> VarName \<Rightarrow> Rules \<Rightarrow> bool"
+  ("'(_, _, _, _') \<leadsto> '(_, _')" 70) where
+  "(e\<^sub>p, {}) \<leadsto> (m, v, \<Sigma>) \<Longrightarrow> (l, e\<^sub>p, Some c, e\<^sub>r) \<leadsto> (v, m ? (condition c ? base l e\<^sub>r))" |
+  "(e\<^sub>p, {}) \<leadsto> (m, v, \<Sigma>) \<Longrightarrow> (l, e\<^sub>p, None, e\<^sub>r) \<leadsto> (v, m ? base l e\<^sub>r)"
 
-inductive generate :: "PatternExpr \<Rightarrow> Condition option \<Rightarrow> PatternExpr \<Rightarrow> VarName \<Rightarrow> Rules \<Rightarrow> bool"
-  ("'(_, _, _') \<leadsto> '(_, _')" 70) where
-  "(e\<^sub>p, {}) \<leadsto> (m, v, \<Sigma>) \<Longrightarrow> (e\<^sub>p, Some c, e\<^sub>r) \<leadsto> (v, m ? (condition c ? base e\<^sub>r))" |
-  "(e\<^sub>p, {}) \<leadsto> (m, v, \<Sigma>) \<Longrightarrow> (e\<^sub>p, None, e\<^sub>r) \<leadsto> (v, m ? base e\<^sub>r)"
+code_pred (modes: i \<Rightarrow> i \<Rightarrow> i \<Rightarrow> i \<Rightarrow> o \<Rightarrow> o \<Rightarrow> bool as generateC) generate .
 
-code_pred (modes: i \<Rightarrow> i \<Rightarrow> i \<Rightarrow> o \<Rightarrow> o \<Rightarrow> bool as generateC) generate .
+definition generateRule :: "RuleLabel \<Rightarrow> PatternExpr \<Rightarrow> Condition option \<Rightarrow> PatternExpr \<Rightarrow> (VarName \<times> Rules)" where
+  "generateRule l p c r = Predicate.the (generateC l p c r)"
 
-definition generateRule :: "PatternExpr \<Rightarrow> Condition option \<Rightarrow> PatternExpr \<Rightarrow> (VarName \<times> Rules)" where
-  "generateRule p c r = Predicate.the (generateC p c r)"
-
-value "Predicate.the (generateC 
+value "Predicate.the (generateC STR ''myrule''
     (BinaryExprPattern BinSub (BinaryExprPattern BinAdd (VariableExprPattern STR ''x'') (VariableExprPattern STR ''y'')) (VariableExprPattern STR ''x''))
     None 
     (VariableExprPattern STR ''x''))"
@@ -1547,7 +1626,7 @@ lemma ground_restriction:
   by (metis restricted)
 
 theorem generate_sound:
-  assumes "(e\<^sub>p, c, e\<^sub>r) \<leadsto> (v, r)"
+  assumes "(l, e\<^sub>p, c, e\<^sub>r) \<leadsto> (v, r)"
   assumes "eval_rules r [v \<mapsto> e\<^sub>g] e"
   assumes "valid_pattern e\<^sub>p"
   assumes "\<L> e\<^sub>r \<subseteq> \<L> e\<^sub>p"
@@ -1558,7 +1637,7 @@ proof -
     using assms(1) generate.simps by blast
   then obtain \<sigma>' where meval: "m \<U> [v \<mapsto> e\<^sub>g] = \<sigma>'"
     by (metis assms(1) assms(2) condE generate.cases lower_deterministic)
-  then have "eval_rules (base e\<^sub>r) \<sigma>' e"
+  then have "eval_rules (base l e\<^sub>r) \<sigma>' e"
     by (smt (verit, ccfv_threshold) assms(1) assms(2) condE eval_match_condition eval_match_deterministic generate.simps lower_deterministic mgen)
   then have e: "e = (e\<^sub>r $$ \<sigma>')"
     using eval_rules.simps by blast
@@ -1835,7 +1914,7 @@ qed
 
 theorem sound_rules:
   assumes "pattern_refinement e\<^sub>r e\<^sub>p"
-  assumes "(e\<^sub>p, c, e\<^sub>r) \<leadsto> (v, r)"
+  assumes "(l, e\<^sub>p, c, e\<^sub>r) \<leadsto> (v, r)"
   assumes "eval_rules r [v \<mapsto> e\<^sub>g] (Some e')"
   assumes "valid_pattern e\<^sub>p"
   assumes "\<L> e\<^sub>r \<subseteq> \<L> e\<^sub>p"
@@ -1858,22 +1937,22 @@ lemma det_variable_match:
   by (smt (verit) MATCH.distinct(17) MATCH.distinct(7) dom_empty dom_fun_upd empty_iff eval_match_noop lower.cases option.distinct(1) singleton_iff)
 
 lemma det_variable_rules:
-  assumes "(e\<^sub>p, c, e\<^sub>r) \<leadsto> (v, r)"
+  assumes "(l, e\<^sub>p, c, e\<^sub>r) \<leadsto> (v, r)"
   assumes "eval_rules r [v' \<mapsto> e\<^sub>g] (Some e')"
   shows "v = v'"
   using assms det_variable_match
   by (smt (verit) Rules.distinct(1) Rules.distinct(11) Rules.distinct(13) Rules.distinct(9) Rules.inject(2) eval_rules.simps generate.simps)
 
 lemma lift_choice:
-  assumes "\<forall> r \<in> set rules. \<exists>e\<^sub>r c e\<^sub>p v. pattern_refinement e\<^sub>r e\<^sub>p \<and> (e\<^sub>p, c, e\<^sub>r) \<leadsto> (v, r) \<and> valid_pattern e\<^sub>p \<and> \<L> e\<^sub>r \<subseteq> \<L> e\<^sub>p \<and> \<L> c \<subseteq> \<L> e\<^sub>p"
+  assumes "\<forall> r \<in> set rules. \<exists>l e\<^sub>r c e\<^sub>p v. pattern_refinement e\<^sub>r e\<^sub>p \<and> (l, e\<^sub>p, c, e\<^sub>r) \<leadsto> (v, r) \<and> valid_pattern e\<^sub>p \<and> \<L> e\<^sub>r \<subseteq> \<L> e\<^sub>p \<and> \<L> c \<subseteq> \<L> e\<^sub>p"
   assumes "eval_rules (choice rules) [v \<mapsto> e\<^sub>g] (Some e')"
   shows "e' \<le> e\<^sub>g"
-  using assms using det_variable_rules
-  by (metis (no_types, lifting) choiceE option.distinct(1) sound_rules)
+  using assms using det_variable_rules choiceE option.distinct(1) sound_rules
+  by (smt (verit))
 
 lemma lift_else:
-  assumes "\<exists>e\<^sub>r c e\<^sub>p v. pattern_refinement e\<^sub>r e\<^sub>p \<and> valid_pattern e\<^sub>p \<and> \<L> e\<^sub>r \<subseteq> \<L> e\<^sub>p \<and> \<L> c \<subseteq> \<L> e\<^sub>p \<and> (e\<^sub>p, c, e\<^sub>r) \<leadsto> (v, r1)"
-  assumes "\<exists>e\<^sub>r c e\<^sub>p v. pattern_refinement e\<^sub>r e\<^sub>p \<and> valid_pattern e\<^sub>p \<and> \<L> e\<^sub>r \<subseteq> \<L> e\<^sub>p \<and> \<L> c \<subseteq> \<L> e\<^sub>p \<and> (e\<^sub>p, c, e\<^sub>r) \<leadsto> (v, r2)"
+  assumes "\<exists>l e\<^sub>r c e\<^sub>p v. pattern_refinement e\<^sub>r e\<^sub>p \<and> valid_pattern e\<^sub>p \<and> \<L> e\<^sub>r \<subseteq> \<L> e\<^sub>p \<and> \<L> c \<subseteq> \<L> e\<^sub>p \<and> (l, e\<^sub>p, c, e\<^sub>r) \<leadsto> (v, r1)"
+  assumes "\<exists>l e\<^sub>r c e\<^sub>p v. pattern_refinement e\<^sub>r e\<^sub>p \<and> valid_pattern e\<^sub>p \<and> \<L> e\<^sub>r \<subseteq> \<L> e\<^sub>p \<and> \<L> c \<subseteq> \<L> e\<^sub>p \<and> (l, e\<^sub>p, c, e\<^sub>r) \<leadsto> (v, r2)"
   assumes "eval_rules (r1 else r2) [v \<mapsto> e\<^sub>g] (Some e')"
   shows "e' \<le> e\<^sub>g"
   using assms using det_variable_rules
@@ -1944,7 +2023,7 @@ locale metaopt =
   assumes size_else: "size r1 < size (either r1 r2) \<and> size r2 < size (either r1 r2)"
   assumes size_choice: "\<forall>r \<in> set rules. size r < size (choice rules)"
   assumes size_cond: "size r < size (cond m r)"
-  assumes size_base: "size (base e) = size (base e)"
+  assumes size_base: "size (base l e) = size (base l e)"
   assumes size_seq: "size r1 < size (seq r1 r2) \<and> size r2 < size (seq r1 r2)"
 begin
 
@@ -1957,7 +2036,7 @@ function apply_meta :: "Rules \<Rightarrow> Rules" where
       (either r1 r2) \<Rightarrow> (either (apply_meta r1) (apply_meta r2)) |
       (choice rules) \<Rightarrow> choice (map (apply_meta) rules) |
       (cond m r) \<Rightarrow> cond m (apply_meta r) |
-      (base e) \<Rightarrow> (base e) |
+      (base l e) \<Rightarrow> (base l e) |
       (seq r1 r2) \<Rightarrow> (seq (apply_meta r1) r2) \<comment> \<open>Avoid recursing through rhs as it could change the entry var\<close>
   ))"
   apply pat_completeness+
@@ -2091,7 +2170,7 @@ qed
 
 fun combined_size :: "Rules \<Rightarrow> nat" where
   "combined_size (m ? r) = 1 + (2 * size m) + combined_size r" |
-  "combined_size (base e) = 0" |
+  "combined_size (base l e) = 0" |
   "combined_size (r1 else r2) = 1 + combined_size r1 + combined_size r2" |
   "combined_size (choice (rule # rules)) = 1 + combined_size rule + combined_size (choice rules)" |
   "combined_size (choice []) = 1" |
@@ -2136,12 +2215,12 @@ fun run where "run x = lift_cond.apply_meta x"
 thm lift_cond.apply_meta_sound
 thm_oracles lift_cond.apply_meta_sound
 
-value "(snd (Predicate.the (generateC 
+value "(snd (Predicate.the (generateC STR ''myrule''
     (BinaryExprPattern BinSub (BinaryExprPattern BinAdd (VariableExprPattern STR ''x'') (VariableExprPattern STR ''y'')) (VariableExprPattern STR ''x''))
     None
     (VariableExprPattern STR ''x''))))"
 
-value "run (snd (Predicate.the (generateC 
+value "run (snd (Predicate.the (generateC STR ''myrule''
     (BinaryExprPattern BinSub (BinaryExprPattern BinAdd (VariableExprPattern STR ''x'') (VariableExprPattern STR ''y'')) (VariableExprPattern STR ''x''))
     None
     (VariableExprPattern STR ''x''))))"
@@ -2269,26 +2348,26 @@ theorem reduce_sound:
   "eval_rules r \<sigma> = eval_rules (reduce r) \<sigma>"
   by (metis comp_eq_dest_lhs join_conditions.apply_meta_sound lift_cond.apply_meta_sound reduce_def)
 
-value "reduce (snd (Predicate.the (generateC 
+value "reduce (snd (Predicate.the (generateC STR ''myrule''
     (BinaryExprPattern BinSub (BinaryExprPattern BinAdd (VariableExprPattern STR ''x'') (VariableExprPattern STR ''y'')) (VariableExprPattern STR ''x''))
     None
     (VariableExprPattern STR ''x''))))"
 
 
 text \<open>Identity\<close>
-value "Predicate.the (generateC 
+value "Predicate.the (generateC STR ''Identity''
   (BinaryExprPattern BinMul (VariableExprPattern STR ''x'') (ConstantExprPattern (IntVal 32 1)))
   None
   (VariableExprPattern STR ''x''))"
 
 text \<open>Eval\<close>
-value "Predicate.the (generateC 
+value "Predicate.the (generateC STR ''Eval''
   (BinaryExprPattern BinMul (ConstantVarPattern STR ''x'') (ConstantVarPattern STR ''y''))
   None
   (ConstantExprPattern (IntVal 32 1)))"
 
 text \<open>Left Shift\<close>
-value "Predicate.the (generateC 
+value "Predicate.the (generateC STR ''Left Shift''
   (BinaryExprPattern BinMul (VariableExprPattern STR ''x'') (ConstantVarPattern STR ''y''))
   (Some (Unary UnaryLogicNegation ((Variable STR ''x'') instanceof ConstantExpr)))
   (BinaryExprPattern BinMul (ConstantVarPattern STR ''y'') (VariableExprPattern STR ''x'')))"
@@ -2339,10 +2418,10 @@ lemma lift_mul:
 context includes match_syntax match_pattern_syntax
 begin
 value "(match STR ''X'' (BinaryPattern BinMul STR ''x'' STR ''Xa'') && match STR ''Xa'' (ConstantPattern (IntVal 32 1)))
-         ? base (VariableExprPattern STR ''x'')"
+         ? base STR '''' (VariableExprPattern STR ''x'')"
 
 value "(match STR ''X'' (BinaryPattern BinMul STR ''Xa'' STR ''Xb'') && match STR ''Xa'' (ConstantVariablePattern STR ''x'')
-        && match STR ''Xb'' (ConstantVariablePattern STR ''y'')) ? base (ConstantVarPattern x)"
+        && match STR ''Xb'' (ConstantVariablePattern STR ''y'')) ? base STR '''' (ConstantVarPattern x)"
 end
 
 
@@ -2484,8 +2563,8 @@ fun export_match :: "MATCH \<Rightarrow> Statement \<Rightarrow> Statement" wher
   "export_match (noop v) r = r"
 
 fun generate_rules :: "VarName option \<Rightarrow> Rules \<Rightarrow> Statement" where
-  "generate_rules None (base e) = return (construct_node e)" |
-  "generate_rules (Some v) (base e) = v := (construct_node e)" |
+  "generate_rules None (base l e) = JavaComment l; return (construct_node e)" |
+  "generate_rules (Some v) (base l e) = JavaComment l; v := (construct_node e)" |
   "generate_rules v (cond m r) = export_match m (generate_rules v r)" |
   "generate_rules v (either r1 r2) = generate_rules v r1; generate_rules v r2" |
   "generate_rules v (choice rules) = JavaSequential (map (generate_rules v) rules)" |
@@ -2502,10 +2581,10 @@ end
 context includes match_syntax match_pattern_syntax
 begin
 value "generate_statement 0 (export ((match STR ''X'' (BinaryPattern BinMul STR ''x'' STR ''Xa'') && match STR ''Xa'' (ConstantPattern (IntVal 32 1)))
-         ? base (VariableExprPattern STR ''x'')))"
+         ? base STR '''' (VariableExprPattern STR ''x'')))"
 
 value "(match STR ''X'' (BinaryPattern BinMul STR ''Xa'' STR ''Xb'') && match STR ''Xa'' (ConstantVariablePattern STR ''x'')
-        && match STR ''Xb'' (ConstantVariablePattern STR ''y'')) ? base (ConstantVarPattern x)"
+        && match STR ''Xb'' (ConstantVariablePattern STR ''y'')) ? base STR '''' (ConstantVarPattern x)"
 end
 (*
   cond MATCH Rules |
