Optimizations/DSL/Canonicalization.thy
@@ -18,6 +18,30 @@ begin
 print_methods
 
 ML \<open>
+fun replaceSubstring (original: string, target: string, replacement: string): string =
+    let
+        val targetLength = String.size target
+        val originalLength = String.size original
+
+        fun replaceHelper (pos: int, acc: string): string =
+            if pos + targetLength <= originalLength then
+                let
+                    val currentSubstr = String.substring (original, pos, targetLength)
+                    val nextChar = String.substring (original, pos, 1)
+                    val updatedAcc = if currentSubstr = target then acc ^ replacement else acc ^ nextChar
+                    val jump = if currentSubstr = target then targetLength else 1
+                in
+                    replaceHelper (pos + jump, updatedAcc)
+                end
+            else
+                acc ^ String.extract (original, pos, NONE)
+
+    in
+        replaceHelper (0, "")
+    end
+\<close>
+
+ML \<open>
 datatype 'a Rewrite =
   Rule of 'a * 'a * term option
 
@@ -240,28 +264,6 @@ definition generate :: "Rules \<Rightarrow> string" where
   "generate = (generate_statement 0) o export"
 
 ML \<open>
-fun replaceSubstring (original: string, target: string, replacement: string): string =
-    let
-        val targetLength = String.size target
-        val originalLength = String.size original
-
-        fun replaceHelper (pos: int, acc: string): string =
-            if pos + targetLength <= originalLength then
-                let
-                    val currentSubstr = String.substring (original, pos, targetLength)
-                    val nextChar = String.substring (original, pos, 1)
-                    val updatedAcc = if currentSubstr = target then acc ^ replacement else acc ^ nextChar
-                    val jump = if currentSubstr = target then targetLength else 1
-                in
-                    replaceHelper (pos + jump, updatedAcc)
-                end
-            else
-                acc ^ String.extract (original, pos, NONE)
-
-    in
-        replaceHelper (0, "")
-    end
-
 fun gencode thy name term =
   let
     val state = Toplevel.make_state (SOME thy);
@@ -271,9 +273,11 @@ fun gencode thy name term =
     ((Const ("Canonicalization.generate", @{typ "Rules \<Rightarrow> string"}))
       $ code);
     val value = Code_Evaluation.dynamic_value_strict ctxt export;
-    val content = Pretty.string_of (Syntax.pretty_term ctxt value);
+    val content = Pretty.unformatted_string_of (Syntax.pretty_term ctxt value);
     val content = replaceSubstring (content, "\<newline>", "\n") (* Replace newlines *)
+    val _ = @{print} content;
     val content = String.substring (content, 2, (String.size content) - 4) (* Strip quotes *)
+    val _ = @{print} content;
 
     val cleaned = YXML.content_of content;
 
